Compare example

examples/sort/CompareMain1.v
@@ -20,11 +20,12 @@ Section PROOF.
 
   Context `{Σ: GRA.t}.
 
-  Variable GlobalStb: list (gname * fspec).
+  Variable GlobalStb: SkEnv.t -> list (gname * fspec).
 
   Section SKENV.
+    Variable skenv: SkEnv.t.
 
-    Definition main_spec: fspec := mk_simple "Main" (X:=unit) 
+    Definition main_spec: fspec := mk_simple "Main" (X:=unit)
                                              (fun _ => (
                                                   (fun _ o => ⌜o = ord_top⌝),
                                                   top2
@@ -32,12 +33,14 @@ Section PROOF.
 
     Definition compare_spec:    fspec := compare_gen mycmp "Main".
 
-    Definition Mainstb: list (gname * fspec) := [("main", main_spec); ("compare", compare_spec)].
+    Definition MainCmpsStb: list (gname * fspec) := [("compare", compare_spec)].
 
-    Definition Mainsbtb: list (gname * fspecbody) := [("main", mk_specbody main_spec (fun _ => APC;; trigger (Choose _))); ("compare", mk_specbody compare_spec (fun _ => trigger (Choose _)))].
+    Definition MainStb: list (gname * fspec) := [("main", main_spec); ("compare", compare_spec)].
+
+    Definition MainSbtb: list (gname * fspecbody) := [("main", mk_specbody main_spec (fun _ => APC;; trigger (Choose _))); ("compare", mk_specbody compare_spec (fun _ => trigger (Choose _)))].
 
     Definition MainSem: ModSem.t := {|
-      ModSem.fnsems := List.map (fun '(fn, body) => (fn, fun_to_tgt GlobalStb fn body)) Mainsbtb;
+      ModSem.fnsems := List.map (fun '(fn, body) => (fn, fun_to_tgt (GlobalStb skenv) fn body)) MainSbtb;
       ModSem.mn := "Main";
       ModSem.initial_mr := ε;
       ModSem.initial_st := tt↑;
@@ -46,7 +49,7 @@ Section PROOF.
   End SKENV.
 
   Definition Main: Mod.t := {|
-    Mod.get_modsem := fun skenv => MainSem;
+    Mod.get_modsem := fun skenv => MainSem skenv;
     Mod.sk := [("compare", Sk.Gfun)];
   |}
   .
