examples/sort/CompareHeader.v
@@ -25,6 +25,6 @@ Definition mycmp (n0 n1: Z): Z :=
 Definition compare_gen `{Σ: GRA.t} (f: Z -> Z -> Z) (mn: mname): fspec :=
   mk_simple mn (X:=Z*Z)
             (fun '(n0, n1) => (
-                 (fun varg o => ⌜varg = [Vint n0; Vint n1]↑ /\ o = ord_pure 0⌝), 
+                 (fun varg o => ⌜varg = [Vint n0; Vint n1]↑ /\ o = ord_pure 0⌝),
                  (fun vret => ⌜vret = (Vint (f n0 n1))↑⌝)
             )).
