examples/sort/Wrap1.v
@@ -7,7 +7,7 @@ Require Import ModSem.
 Require Import Skeleton.
 Require Import PCM.
 Require Import HoareDef.
-Require Import MutHeader.
+Require Import CompareHeader.
 Require Import Logic.
 
 Generalizable Variables E R A B C X Y Σ.
@@ -20,24 +20,25 @@ Section PROOF.
 
   Context `{Σ: GRA.t}.
 
-  Variable cmpspecs: list (gname * (Z -> Z -> Z)).
+  Variable CmpsStb: SkEnv.t -> list (gname * fspec).
   Variable GlobalStb: SkEnv.t -> list (gname * fspec).
 
   Section SKENV.
     Variable skenv: SkEnv.t.
 
+    (* TODO: define (myfind: list (string * A) -> A -> option A) and use it *)
     Definition wrap_spec:    fspec := mk_simple "Wrap" (X:=Z*Z*(Z -> Z -> Z))
                                                 (fun '(n0, n1, f) => (
-                                                     (fun varg o => ⌜exists fn blk, varg = [Vint n0; Vint n1; Vptr blk 0]↑ /\ o = ord_pure 1 /\ skenv.(SkEnv.blk2id) blk = Some fn /\ List.find (fun '(_fn, _) => dec fn _fn) cmpspecs = Some (fn, f)⌝), 
+                                                     (fun varg o => ⌜exists fn blk, varg = [Vint n0; Vint n1; Vptr blk 0]↑ /\ o = ord_pure 1 /\ skenv.(SkEnv.blk2id) blk = Some fn /\ List.find (fun '(_fn, _) => dec fn _fn) (CmpsStb skenv) = Some (fn, compare_gen f fn)⌝),
                                                      (fun vret => ⌜vret = (Vint (f n0 n1))↑⌝)
                                                 )).
 
-    Definition Wrapstb: list (gname * fspec) := [("wrap", wrap_spec)].
+    Definition WrapStb: list (gname * fspec) := [("wrap", wrap_spec)].
 
-    Definition Wrapsbtb: list (gname * fspecbody) := [("wrap", mk_specbody wrap_spec (fun _ => trigger (Choose _)))].
+    Definition WrapSbtb: list (gname * fspecbody) := [("wrap", mk_specbody wrap_spec (fun _ => trigger (Choose _)))].
 
     Definition WrapSem: ModSem.t := {|
-      ModSem.fnsems := List.map (fun '(fn, body) => (fn, fun_to_tgt (GlobalStb skenv) fn body)) Wrapsbtb;
+      ModSem.fnsems := List.map (fun '(fn, body) => (fn, fun_to_tgt (GlobalStb skenv) fn body)) WrapSbtb;
       ModSem.mn := "Wrap";
       ModSem.initial_mr := ε;
       ModSem.initial_st := tt↑;
@@ -52,6 +53,3 @@ Section PROOF.
   .
 
 End PROOF.
-
-(* Definition cmpspecs: gname -> option (Z -> Z -> Z) := *)
-(*   fun fn => option_map snd (List.find (fun '(str, _) => eqb str fn) [("compare", mycmp)]). *)
